Clean up all 3 existing axiomatic models
- Better barrier classification section
- Use standardized event sets
- Make all models depend on a register whitelist
- Make all models take in a register whitelist

AxiomaticModels/GenAxiomaticArm.v
@@ -4,7 +4,7 @@ Require Import SSCCommon.GRel.
 Require Import SSCCommon.FMon.
 Require Import GenModels.ArmInst.
 
-(* NOTE:
+(* NOTE: TODO change this.
  This file defines the VMSA and User Arm axiomatic models. It starts with some
  common definitions (in section common_def), followed by module GenArm which
  contains a candidate cd, an inital memory map init_mem, with preliminary common
@@ -13,490 +13,146 @@ Require Import GenModels.ArmInst.
  dependencies between the two models.
  *)
 
-Section common_def.
-  Import Candidate.
 
+(** * Definition of barriers categories and barrier sets
+
+      This section defines the event sets of Arm barrier and the corresponding
+      classification. For now only dmbs, dsbs and isbs are supported.
+
+      This development assumes that all hardware threads are in the same inner
+      shareability domain, therefore we identify barriers that are:
+      - Full system
+      - Outer shareable
+      - Inner shareable
+      This might need to change when considering device interaction later *)
+Section Barriers.
+  Import Candidate.
+  Context {et : exec_type} {nmth : nat}.
+  Implicit Type cd : (t et nmth).
+  Implicit Type b : barrier.
   #[local] Hint Extern 10 (Decision (?x _)) => unfold x : typeclass_instances.
   #[local] Hint Extern 10 (Decision (?x _ _)) => unfold x : typeclass_instances.
   #[local] Hint Extern 10 (Decision (?x _ _ _)) => unfold x : typeclass_instances.
 
-  (*** barriers *)
-  (* armv9-interface/barriers.cat *)
-  Implicit Type b : SailArmInstTypes.Barrier.
 
-  Definition is_barrier_P P `{forall b, Decision (P b)} (event : iEvent) :=
-    match event with
-    | Barrier b &→ _ => P b
-    | _ => False
-    end.
+  Definition is_isb b := if b is Barrier_ISB _ then True else False.
+  Definition isb cd := collect_all (λ _, is_barrierP is_isb) cd.
 
-  Global Instance is_barrier_P_dec P `{forall b, Decision (P b)} event :
-    Decision (is_barrier_P P event).
-  Proof. apply _. Qed.
+  Definition is_dsbP (P : MBReqTypes → Prop) b :=
+    if b is Barrier_DSB dxb
+    then dxb.(DxB_domain) ≠ MBReqDomain_Nonshareable ∧ P dxb.(DxB_types)
+    else False.
+  Definition is_dsb := is_dsbP (λ _, True).
+  Definition is_dsbT t := is_dsbP (.=t).
 
-  Definition is_isb (barrier : barrier) :=
-    match barrier with
-    | Barrier_ISB _ => True
-    | _ => False
-    end.
+  Definition is_dsbnshP (P : MBReqTypes → Prop) b :=
+    if b is Barrier_DSB dxb
+    then dxb.(DxB_domain) = MBReqDomain_Nonshareable ∧ P dxb.(DxB_types)
+    else False.
+  Definition is_dsbnsh := is_dsbnshP (λ _, True).
+  Definition is_dsbnshT t := is_dsbnshP (.=t).
 
-  Definition isb {et n} (cd : Candidate.t et n) :=
-    collect_all (λ _ event, is_barrier_P is_isb event) cd.
+  Definition dsbsy cd :=
+    collect_all (λ _, is_barrierP (is_dsbT MBReqTypes_All)) cd.
+  Definition dsbst cd :=
+    collect_all (λ _, is_barrierP (is_dsbT MBReqTypes_Writes)) cd.
+  Definition dsbld cd :=
+    collect_all (λ _, is_barrierP (is_dsbT MBReqTypes_Reads)) cd.
+  Definition dsb cd := collect_all (λ _, is_barrierP is_dsb) cd.
+  Definition dsbnshsy cd :=
+    collect_all (λ _, is_barrierP (is_dsbnshT MBReqTypes_All)) cd.
+  Definition dsbnshst cd :=
+    collect_all (λ _, is_barrierP (is_dsbnshT MBReqTypes_Writes)) cd.
+  Definition dsbnshld cd :=
+    collect_all (λ _, is_barrierP (is_dsbnshT MBReqTypes_Reads)) cd.
+  Definition dsbnsh cd := collect_all (λ _, is_barrierP is_dsbnsh) cd.
 
-  Definition has_dsb_P P `{forall dxb, Decision (P dxb)} (barrier : barrier) :=
-    match barrier with
-    | Barrier_DSB dxb => P dxb
-    | _ => False
-    end.
+  Definition is_dmbP (P : MBReqTypes → Prop) b :=
+    if b is Barrier_DMB dxb
+    then dxb.(DxB_domain) ≠ MBReqDomain_Nonshareable ∧ P dxb.(DxB_types)
+    else False.
+  Definition is_dmb := is_dmbP (λ _, True).
+  Definition is_dmbT t := is_dmbP (.=t).
 
-  Global Instance has_dsb_P_dec P `{forall dxb, Decision (P dxb)} barrier :
-    Decision (has_dsb_P P barrier).
-  Proof. apply _. Qed.
+  Definition is_dmbnshP (P : MBReqTypes → Prop) b :=
+    if b is Barrier_DMB dxb
+    then dxb.(DxB_domain) = MBReqDomain_Nonshareable ∧ P dxb.(DxB_types)
+    else False.
+  Definition is_dmbnsh := is_dmbnshP (λ _, True).
+  Definition is_dmbnshT t := is_dmbnshP (.=t).
 
-  Definition is_dsbsy := has_dsb_P
-                           (λ dxb,
-                              (* DSBISH *)
-                              (dxb.(DxB_domain) = MBReqDomain_InnerShareable
-                               ∧ dxb.(DxB_types) = MBReqTypes_All)
-                              (* DSBSY *)
-                              ∨ (dxb.(DxB_domain) = MBReqDomain_FullSystem
-                                 ∧ dxb.(DxB_types) = MBReqTypes_All)
-                              (* DSBNSH *)
-                              ∨ (dxb.(DxB_domain) = MBReqDomain_Nonshareable
-                                 ∧ dxb.(DxB_types) = MBReqTypes_All)
-                           ).
+  Definition dmbsy cd :=
+    collect_all (λ _, is_barrierP (is_dmbT MBReqTypes_All)) cd.
+  Definition dmbst cd :=
+    collect_all (λ _, is_barrierP (is_dmbT MBReqTypes_Writes)) cd.
+  Definition dmbld cd :=
+    collect_all (λ _, is_barrierP (is_dmbT MBReqTypes_Reads)) cd.
+  Definition dmb cd := collect_all (λ _, is_barrierP is_dmb) cd.
+  Definition dmbnshsy cd :=
+    collect_all (λ _, is_barrierP (is_dmbnshT MBReqTypes_All)) cd.
+  Definition dmbnshst cd :=
+    collect_all (λ _, is_barrierP (is_dmbnshT MBReqTypes_Writes)) cd.
+  Definition dmbnshld cd :=
+    collect_all (λ _, is_barrierP (is_dmbnshT MBReqTypes_Reads)) cd.
+  Definition dmbnsh cd := collect_all (λ _, is_barrierP is_dmbnsh) cd.
 
-  Global Instance is_dsbsy_dec dxb : Decision (is_dsbsy dxb).
-  Proof. apply _. Qed.
+  (** ** Cumulated barriers
 
-  (* armv9-interface/barriers.cat#L112 *)
-  Definition dsbsy {et n} (cd : Candidate.t et n) :=
-    collect_all (λ _ event, is_barrier_P is_dsbsy event) cd.
+      Each of those set collect all barrier that are stronger than the set name *)
 
-  Definition is_dsbst b := is_dsbsy b
-                           ∨ (has_dsb_P
-                                (λ dxb,
-                                   (* DSBST *)
-                                   (dxb.(DxB_types) = MBReqTypes_Writes)
-                                   (* DSBISHST *)
-                                   ∨ (dxb.(DxB_domain) = MBReqDomain_InnerShareable
-                                      ∧ dxb.(DxB_types) = MBReqTypes_Writes)
-                                   (* DSBNSHST *)
-                                   ∨ (dxb.(DxB_domain) = MBReqDomain_Nonshareable
-                                      ∧ dxb.(DxB_types) = MBReqTypes_Writes)
-                                ) b).
+  Definition dsb_full cd := dsbsy cd.
+  Definition dsb_load cd := dsbld cd ∪ dsbsy cd.
+  Definition dsb_store cd := dsbst cd ∪ dsbsy cd.
+  Definition dmb_full cd := dmbsy cd ∪ dsbsy cd.
+  Definition dmb_load cd := dmbld cd ∪ dmbsy cd ∪ dsb_load cd.
+  Definition dmb_store cd := dmbst cd ∪ dmbsy cd ∪ dsb_store cd.
 
-  Global Instance is_dsbst_dec dxb : Decision (is_dsbst dxb).
-  Proof. apply _. Qed.
+End Barriers.
 
-  (* armv9-interface/barriers.cat#L115 *)
-  Definition dsbst {et n} (cd : Candidate.t et n) :=
-    collect_all (λ _ event, is_barrier_P is_dsbst event) cd.
-
-  Definition is_dsbld b := is_dsbsy b
-                           ∨ (has_dsb_P
-                                (λ dxb,
-                                   (* DSBLD *)
-                                   (dxb.(DxB_types) = MBReqTypes_Reads)
-                                   (* DSBISHLD *)
-                                   ∨ (dxb.(DxB_domain) = MBReqDomain_InnerShareable
-                                      ∧ dxb.(DxB_types) = MBReqTypes_Reads)
-                                   (* DSBNSHLD *)
-                                   ∨ (dxb.(DxB_domain) = MBReqDomain_Nonshareable
-                                      ∧ dxb.(DxB_types) = MBReqTypes_Reads)
-                                ) b).
-
-  Global Instance is_dsbld_dec dxb : Decision (is_dsbld dxb).
-  Proof. apply _. Qed.
-
-  (* armv9-interface/barriers.cat#L115 *)
-  Definition dsbld {et n} (cd : Candidate.t et n) :=
-    collect_all (λ _ event, is_barrier_P is_dsbld event) cd.
-
-  Definition is_dsbnsh := has_dsb_P
-                            (λ dxb,
-                               (* DSBNSH *)
-                               (dxb.(DxB_domain) = MBReqDomain_InnerShareable
-                                ∧ dxb.(DxB_types) = MBReqTypes_All)).
-
-  Global Instance is_dsbnsh_dec dxb : Decision (is_dsbnsh dxb).
-  Proof. apply _. Qed.
-
-  (* armv9-interface/barriers.cat#L121 *)
-  Definition dsbnsh {et n} (cd : Candidate.t et n) :=
-    collect_all (λ _ event, is_barrier_P is_dsbnsh event) cd.
-
-
-  Definition has_dmb_P P `{forall dxb, Decision (P dxb)} (barrier : barrier) :=
-    match barrier with
-    | Barrier_DMB dxb => P dxb
-    | _ => False
-    end.
-
-  Global Instance has_dmb_P_dec P `{forall dxb, Decision (P dxb)} barrier :
-    Decision (has_dmb_P P barrier).
-  Proof. apply _. Qed.
-
-  Definition is_dmbsy b := is_dsbsy b
-                           ∨ (has_dmb_P
-                                (λ dxb,
-                                   (* DMBSY *)
-                                   (dxb.(DxB_domain) = MBReqDomain_FullSystem
-                                    ∧ dxb.(DxB_types) = MBReqTypes_All)
-                                   (* DMBISH *)
-                                   ∨ (dxb.(DxB_domain) = MBReqDomain_InnerShareable
-                                      ∧ dxb.(DxB_types) = MBReqTypes_All)
-                                   (* DMBNSH *)
-                                   ∨ (dxb.(DxB_domain) = MBReqDomain_Nonshareable
-                                      ∧ dxb.(DxB_types) = MBReqTypes_All)
-                                ) b).
-
-  Global Instance is_dmbsy_dec dxb : Decision (is_dmbsy dxb).
-  Proof. apply _. Qed.
-
-  (* armv9-interface/barriers.cat#L124 *)
-  Definition dmbsy {et n} (cd : Candidate.t et n) :=
-    collect_all (λ _ event, is_barrier_P is_dmbsy event) cd.
-
-  Definition is_dmbst b := is_dmbsy b ∨ is_dsbst b
-                           ∨ (has_dmb_P
-                                (λ dxb,
-                                   (* DMBST *)
-                                   (dxb.(DxB_domain) = MBReqDomain_FullSystem
-                                    ∧ dxb.(DxB_types) = MBReqTypes_Writes)
-                                   (* DMBISHST *)
-                                   ∨ (dxb.(DxB_domain) = MBReqDomain_InnerShareable
-                                      ∧ dxb.(DxB_types) = MBReqTypes_Writes)
-                                   (* DMBNSHST *)
-                                   ∨ (dxb.(DxB_domain) = MBReqDomain_Nonshareable
-                                      ∧ dxb.(DxB_types) = MBReqTypes_Writes)
-                                ) b).
-
-  Global Instance is_dmbst_dec dxb : Decision (is_dmbst dxb).
-  Proof. apply _. Qed.
-
-  (* armv9-interface/barriers.cat#L127 *)
-  Definition dmbst {et n} (cd : Candidate.t et n) :=
-    collect_all (λ _ event, is_barrier_P is_dmbst event) cd.
-
-  Definition is_dmbld b := is_dmbsy b ∨ is_dsbld b
-                           ∨ (has_dmb_P
-                                (λ dxb,
-                                   (* DMBLD *)
-                                   (dxb.(DxB_domain) = MBReqDomain_FullSystem
-                                    ∧ dxb.(DxB_types) = MBReqTypes_Reads)
-                                   (* DMBISHLD *)
-                                   ∨ (dxb.(DxB_domain) = MBReqDomain_InnerShareable
-                                      ∧ dxb.(DxB_types) = MBReqTypes_Reads)
-                                   (* DMBNSHLD *)
-                                   ∨ (dxb.(DxB_domain) = MBReqDomain_Nonshareable
-                                      ∧ dxb.(DxB_types) = MBReqTypes_Reads)
-                                ) b).
-
-  Global Instance is_dmbld_dec dxb : Decision (is_dmbld dxb).
-  Proof. apply _. Qed.
-
-  (* armv9-interface/barriers.cat#L130 *)
-  Definition dmbld {et n} (cd : Candidate.t et n) :=
-    collect_all (λ _ event, is_barrier_P is_dmbld event) cd.
-
-  Definition is_dmb b := is_dmbsy b ∨ is_dmbst b ∨ is_dmbld b.
-
-  Global Instance is_dmb_dec dxb : Decision (is_dmb dxb).
-  Proof. apply _. Qed.
-
-  (* armv9-interface/barriers.cat#L133 *)
-  Definition dmb {et n} (cd : Candidate.t et n) :=
-    collect_all (λ _ event, is_barrier_P is_dmb event) cd.
-
-  Definition is_dsb b := is_dsbsy b ∨ is_dsbst b ∨ is_dsbld b.
-
-  Global Instance is_dsb_dec dxb : Decision (is_dsb dxb).
-  Proof. apply _. Qed.
-
-  (* armv9-interface/barriers.cat#L136 *)
-  Definition dsb {et n} (cd : Candidate.t et n) :=
-    collect_all (λ _ event, is_barrier_P is_dsb event) cd.
-
-
-  Definition is_explicit_access_kind_P P (event : iEvent) : Prop :=
-    match event with
-    | MemRead _ rreq &→ _ => match rreq.(ReadReq.access_kind) with
-                                  | AK_explicit ak => P ak
-                                  | _ => False
-                                  end
-    | MemWrite _ wreq &→ _ => match wreq.(WriteReq.access_kind) with
-                                   | AK_explicit ak => P ak
-                                   | _ => False
-                                   end
-    | _ => False
-    end.
+Module AxArmNames.
+  Import Candidate.
+  Section ArmNames.
 
   Context {et : exec_type} {nmth : nat}.
   Context `(cd : t et nmth).
 
-  (*** interface-common *)
-
-  (* interface-common.cat#L2 *)
   Definition F := barriers cd.
 
-  (* interface-common.cat#L6 *)
-  (* explicit writes *)
-  Definition W :=
-    collect_all (λ _ event, is_mem_write event
-                            ∧ is_explicit_access_kind_P (λ _, True) event) cd.
+  Definition W := explicit_writes cd.
+  Definition R := explicit_reads cd.
+  Definition Wx := exclusive_writes cd.
+  Definition Rx := exclusive_writes cd.
+  Definition L := rel_acq_writes cd.
+  Definition A := rel_acq_reads cd.
+  Definition Q := acq_rcpc_reads cd.
+  Definition T := ttw_reads cd.
 
-  (* interface-common.cat#L5 *)
-  Definition R :=
-    collect_all (λ _ event, is_mem_read event
-                            ∧ is_explicit_access_kind_P (λ _, True) event) cd.
-
-  (* interface-common.cat#L52 *)
-  Definition L :=
-    collect_all
-      (λ _ event, is_mem_write event
-                  ∧ is_explicit_access_kind_P
-                      (λ ak, ak.(Explicit_access_kind_strength) = AS_rel_or_acq)
-                      event) cd.
-
-  (* interface-common.cat#L46 *)
-  Definition A :=
-    collect_all
-      (λ _ event, is_mem_read event
-                  ∧ is_explicit_access_kind_P
-                      (λ ak, ak.(Explicit_access_kind_strength) = AS_rel_or_acq)
-                      event) cd.
-
-  (* interface-common.cat#L49 *)
-  Definition Q :=
-    collect_all
-      (λ _ event, is_mem_read event
-                  ∧ is_explicit_access_kind_P
-                      (λ ak, ak.(Explicit_access_kind_strength) = AS_acq_rcpc)
-                      event) cd.
-
-  Definition is_tlbi (event : iEvent) :=
-    match event with
-    | TlbOp _ &→ _ => True
-    | _ => False
-    end.
-
-  Global Instance is_tlbi_dec event : Decision (is_tlbi event).
-  Proof. apply _. Qed.
-
-  Definition is_cacheop (event : iEvent) :=
-    match event with
-    | CacheOp _ &→ _ => True
-    | _ => False
-    end.
-
-  Global Instance is_cacheop_dec event : Decision (is_cacheop event).
-  Proof. unfold is_cacheop. apply _. Qed.
-
-  (* interface-common.cat#L65 *)
-  Definition C := collect_all (λ _ event, is_tlbi event ∨ is_cacheop event) cd.
-
-  (* interface-common.cat#L68 *)
-  Definition TLBI := collect_all (λ _ event, is_tlbi event) cd.
-
-  Definition is_take_exception (event : iEvent) :=
-    match event with
-    | TakeException _ &→ _ => True
-    | _ => False
-    end.
-
-  Global Instance is_take_exception_dec event : Decision (is_take_exception event).
-  Proof. apply _. Qed.
-
-  (* interface-common.cat#L71 *)
+  (* All cache flushing operations *)
+  Definition C := collect_all (λ _ ev, is_tlbop ev ∨ is_cacheop ev) cd.
+  Definition TLBI := collect_all (λ _ ev, is_tlbop ev) cd.
   Definition TE := collect_all (λ _ event, is_take_exception event) cd.
-
-  Definition is_return_exception (event : iEvent) :=
-    match event with
-    | ReturnException &→ _ => True
-    | _ => False
-    end.
-
-  Global Instance is_return_exception_dec event :
-    Decision (is_return_exception event).
-  Proof. apply _. Qed.
-
-  (* interface-common.cat#L72 *)
   Definition ERET := collect_all (λ _ event, is_return_exception event) cd.
 
-  (*** regs *)
+  Definition is_msr := is_reg_writeP (λ _ o _, is_Some o).
+  Definition MSR := collect_all (λ _, is_msr) cd.
 
-  (* armv9-interface/regs.cat#L2 *)
-  Definition is_msr (event : iEvent) :=
-    match event with
-    | RegWrite _ (Some _) _ &→ _ => True
-    | _ => False
-  end.
-  Global Instance is_msr_dec event : Decision (is_msr event).
-  Proof. unfold is_msr. apply _. Qed.
-
-  Definition MSR := collect_all (λ _ event, is_msr event) cd.
-
-  (* translation-table-walk reads *)
-  Definition is_translate (event : iEvent) :=
-    match event with
-    | MemRead _ rreq &→ _ => rreq.(ReadReq.access_kind) = AK_ttw ()
-    | _ => False
-    end.
-
-  Global Instance is_translate_dec event : Decision (is_translate event).
-  Proof. apply _. Qed.
-
-  (* translation-common.cat#L9 *)
-  Definition T := collect_all (λ _ event, is_translate event) cd.
 
   (* A MemRead with ttw and value 0 *)
-  Definition is_translation_read_fault (event : iEvent) :=
-    match event with
-    | MemRead n rreq &→ resp =>
-        match rreq.(ReadReq.access_kind), resp with
-        | AK_ttw (), inl (val, _) => val = bv_0 _
-        | _, _ => False
-        end
-    | _ => False
-    end.
-
-  Global Instance is_translation_fault_dec event :
-    Decision (is_translation_read_fault event).
-  Proof.
-    unfold is_translation_read_fault.
-    destruct event as [call ret].
-    destruct call; tc_solve.
-  Qed.
+  Definition is_translation_read_fault :=
+    is_mem_readP (λ n rr val _, is_ttw rr.(ReadReq.access_kind) ∧ bv_extract 0 1 val = 0%bv).
 
   (* translation-common.cat#L10 *)
   Definition T_f := collect_all (λ _ event, is_translation_read_fault event) cd.
+  Typeclasses Opaque T_f.
 
-  Notation "'lxsx'" := (lxsx cd).
-  Notation "'amo'" := (atomic_update cd).
-  Notation "'addr'" := (addr cd).
-  Notation "'data'" := (data cd).
-  Notation "'ctrl'" := (ctrl cd).
-  Notation "'loc'" := (same_pa cd).
-  (* all mem events (explicit and translation) *)
-  Notation "'writes'" := (mem_writes cd).
-  (* all mem events (explicit and translation) *)
-  Notation "'reads'" := (mem_reads cd).
+  Lemma T_f_in_T : T_f ⊆ T.
+  Proof.
+    unfold T_f, T, ttw_reads, reads_by_kind.
+    set_unfold. hauto q:on use:is_mem_readP_spec.
+  Qed.
 
-  (* will diverge from loc if merging events *)
-  Definition overlap_loc := loc.
+  Definition amo := atomic_update cd.
 
-  Definition rmw := lxsx ∪ amo.
-
-  (* translation-common.cat#L25 *)
-  Notation "'iio'" := (iio cd).
-  (* instruction_order orders events between instructions *)
-  (* translation-common.cat#L26 *)
-  Notation "'instruction_order'" := (instruction_order cd).
-
-End common_def.
-
-Module GenArmNMS.
-  Import Candidate.
-
-  Section def.
-    Context {nmth : nat}.
-    Context (cd : Candidate.t NMS nmth).
-  Notation "'amo'" := (atomic_update cd).
-  Notation "'lxsx'" := (lxsx cd).
-  Notation "'iio'" := (iio cd).
-  Notation "'loc'" := (same_pa cd).
-  Notation "'addr'" := (addr cd).
-  Notation "'data'" := (data cd).
-  Notation "'ctrl'" := (ctrl cd).
-  Notation "'instruction_order'" := (instruction_order cd).
-  Notation "'W'" := (W cd).
-  Notation "'R'" := (R cd).
-
-  Global Instance is_explicit_access_kind_dec P `{forall ak, Decision (P ak)} event :
-    Decision (is_explicit_access_kind_P P event).
-  Proof. unfold is_explicit_access_kind_P. apply _. Qed.
-
-  Definition Wx :=
-    collect_all
-      (λ _ event, is_mem_write event
-                  ∧ is_explicit_access_kind_P
-                      (λ ak, ak.(Explicit_access_kind_variety) = AV_exclusive)
-                      event) cd.
-
-  Definition Rx :=
-    collect_all
-      (λ _ event, is_mem_read event
-                  ∧ is_explicit_access_kind_P
-                      (λ ak, ak.(Explicit_access_kind_variety) = AV_exclusive)
-                      event) cd.
-
-  Export NMSWF.
-
-  Record amo_wf := {
-      amo_dom : grel_dom amo ⊆ Rx;
-      amo_rng : grel_rng amo ⊆ Wx;
-      amo_in_iio : amo ⊆ iio;
-      amo_func : grel_functional amo;
-      amo_inv_func : grel_functional (amo⁻¹);
-      amo_loc : amo ⊆ loc;
-    }.
-
-  Record lxsx_wf := {
-      lxsx_dom : grel_dom lxsx ⊆ Rx;
-      lxsx_rng : grel_rng lxsx ⊆ Wx;
-      lxsx_func : grel_functional lxsx;
-      lxsx_inv_func : grel_functional (lxsx⁻¹);
-      lxsx_loc : lxsx ⊆ loc;
-      lxsx_po : lxsx ⊆ instruction_order;
-    }.
-
-  Record addr_wf :=
-    {
-      addr_dom : grel_dom addr ⊆ R;
-      addr_rng : grel_rng addr ⊆ R ∪ W;
-      addr_in_instruction_order : addr ⊆ instruction_order;
-    }.
-
-  Record data_wf :=
-    {
-      data_dom : grel_dom data ⊆ R;
-      data_rng : grel_rng data ⊆ W;
-      data_in_instruction_order : data ⊆ instruction_order;
-    }.
-
-  Record ctrl_wf :=
-    {
-      ctrl_dom : grel_dom ctrl ⊆ R;
-      ctrl_in_instruction_order : ctrl ⊆ instruction_order;
-      ctrl_instruction_order_in_ctrl : ctrl⨾instruction_order ⊆ ctrl;
-    }.
-
-  Record wellformed:= {
-      amo :> amo_wf;
-      lxsx :> lxsx_wf;
-      full_instruction_order :> NMSWF.full_instruction_order_wf' cd;
-      addr :> addr_wf;
-      data :> data_wf;
-      ctrl :> ctrl_wf;
-    }.
-
-  (* from promising *)
-  Definition get_init_val (a : pa) (init_mem : memoryMap) :=
-    list_from_func 8
-      (fun n => a |> set FullAddress_address (bv_add (Z_to_bv 52 (Z.of_nat n))))
-      |> map init_mem |> bv_of_bytes 64.
-
-  Definition is_initial event init_mem :=
-    (match get_pa event, NMSWF.get_val event with
-     | Some pa, Some val => (get_init_val pa init_mem) = val
-     | _, _ => False
-     end).
-
-  Global Instance is_initial_dec event init_mem :
-    Decision (is_initial event init_mem).
-  Proof. unfold is_initial. apply _. Qed.
-
-  End def.
-
-End GenArmNMS.
+  Definition rmw := lxsx cd ∪ amo.
+  End ArmNames.
+End AxArmNames.
